size classes = {16, 32} \cup [64,2048]
previously, only powers of two
some admits remaining

src/SlotsAlloc.fst
@@ -27,7 +27,7 @@ let slot_array (size_class: sc) (arr: array U8.t) (pos: U32.t)
   : Pure (array U8.t)
   (requires
     U32.v pos < U32.v (nb_slots size_class) /\
-    A.length arr = U32.v page_size)
+    A.length arr >= US.v (rounding size_class))
   (ensures fun r ->
     A.length r == U32.v size_class /\
     same_base_array r arr)
@@ -46,14 +46,14 @@ let slot_array (size_class: sc) (arr: array U8.t) (pos: U32.t)
 
 let slot_vprop
   (size_class: sc)
-  (arr: array U8.t{A.length arr = U32.v page_size})
+  (arr: array U8.t{A.length arr = US.v (rounding size_class)})
   (pos: U32.t{U32.v pos < U32.v (nb_slots size_class)})
   =
   A.varray (slot_array size_class arr pos)
 
 let slot_vprop_lemma
   (size_class: sc)
-  (arr: array U8.t{A.length arr = U32.v page_size})
+  (arr: array U8.t{A.length arr = US.v (rounding size_class)})
   (pos: U32.t{U32.v pos < U32.v (nb_slots size_class)})
   : Lemma
   (t_of (slot_vprop size_class arr pos) == Seq.lseq U8.t (U32.v size_class))
@@ -63,7 +63,7 @@ let slot_vprop_lemma
 let slab_vprop_aux_f
   (size_class: sc)
   (md_as_seq: Seq.lseq U64.t 4)
-  (arr: array U8.t{A.length arr = U32.v page_size})
+  (arr: array U8.t{A.length arr = US.v (rounding size_class)})
   (i: U32.t{U32.v i < U32.v (nb_slots size_class)})
   : vprop
   =
@@ -74,7 +74,7 @@ let slab_vprop_aux_f
 let slab_vprop_aux_f_lemma
   (size_class: sc)
   (md_as_seq: Seq.lseq U64.t 4)
-  (arr: array U8.t{A.length arr = U32.v page_size})
+  (arr: array U8.t{A.length arr = US.v (rounding size_class)})
   : (i: U32.t{U32.v i < U32.v (nb_slots size_class)}) ->
     Lemma (
       t_of (slab_vprop_aux_f size_class md_as_seq arr i)
@@ -88,7 +88,7 @@ let slab_vprop_aux_f_lemma
 
 let slab_vprop_aux
   (size_class: sc)
-  (arr: array U8.t{A.length arr = U32.v page_size})
+  (arr: array U8.t{A.length arr = US.v (rounding size_class)})
   (md_as_seq: Seq.lseq U64.t 4)
   : vprop
   =
@@ -103,7 +103,7 @@ let slab_vprop_aux
 
 let slab_vprop_aux_lemma
   (size_class: sc)
-  (arr: array U8.t{A.length arr = U32.v page_size})
+  (arr: array U8.t{A.length arr = US.v (rounding size_class)})
   (md_as_seq: Seq.lseq U64.t 4)
   : Lemma
   (t_of (slab_vprop_aux size_class arr md_as_seq)
@@ -133,7 +133,9 @@ let slab_vprop
   vrefinedep
     (A.varray md)
     (fun (md_as_seq: Seq.lseq U64.t 4) -> slab_vprop_aux2 size_class md_as_seq)
-    (fun (md_as_seq: Seq.lseq U64.t 4) -> slab_vprop_aux size_class arr md_as_seq)
+    (fun (md_as_seq: Seq.lseq U64.t 4) -> slab_vprop_aux size_class (A.split_l arr (rounding size_class)) md_as_seq)
+  `star`
+  A.varray (A.split_r arr (rounding size_class))
 
 let slab_vprop_lemma
   (size_class: sc)
@@ -142,35 +144,44 @@ let slab_vprop_lemma
   : Lemma
   (t_of (slab_vprop size_class arr md)
   ==
-  dtuple2
-    (x:Seq.lseq U64.t 4{slab_vprop_aux2 size_class x})
-    (fun _ -> Seq.lseq (G.erased (option (Seq.lseq U8.t (U32.v size_class)))) (U32.v (nb_slots size_class))))
-  = let aux (n1 n2:nat) (p:Seq.lseq U64.t n1 -> prop) : Lemma
-      (requires n1 == n2)
-      (ensures (x:Seq.lseq U64.t n1{p x}) == (x:Seq.lseq U64.t n2{p x}))
-    = () in
-    let aux2 (a a':Type) (b c:Type) : Lemma
-      (requires a == a' /\ b == c)
-      (ensures dtuple2 a (fun _ -> b) == dtuple2 a' (fun _ -> c))
-    = () in
-    // The SMT solver needs some help to prove type equality, with rewritings deep in the terms.
-    // In particular, it does not seem to be able to apply the rewritings for aux and aux2 without
-    // explicit calls to the lemmas when they occur under dtuple2
-    assert_norm (
-      t_of (slab_vprop size_class arr md)
-      ==
-      dtuple2
-        (x:Seq.lseq U64.t (A.length md){slab_vprop_aux2 size_class x})
-        (fun _ -> Seq.lseq (G.erased (option (Seq.lseq U8.t (U32.v size_class))))
-          (Seq.length (SeqUtils.init_u32_refined (UInt32.v (nb_slots size_class))))));
-    aux (A.length md) 4 (slab_vprop_aux2 size_class);
-    aux2
-      (x:Seq.lseq U64.t (A.length md){slab_vprop_aux2 size_class x})
+    dtuple2
       (x:Seq.lseq U64.t 4{slab_vprop_aux2 size_class x})
-      (Seq.lseq (G.erased (option (Seq.lseq U8.t (U32.v size_class))))
-        (Seq.length (SeqUtils.init_u32_refined (UInt32.v (nb_slots size_class)))))
-      (Seq.lseq (G.erased (option (Seq.lseq U8.t (U32.v size_class))))
-        (U32.v (nb_slots size_class)))
+      (fun _ -> Seq.lseq (G.erased (option (Seq.lseq U8.t (U32.v size_class)))) (U32.v (nb_slots size_class)))
+    &
+    Seq.lseq U8.t (U32.v page_size - US.v (rounding size_class))
+  )
+  =
+  admit ()
+
+  //let aux (n1 n2:nat) (p:Seq.lseq U64.t n1 -> prop) : Lemma
+  //    (requires n1 == n2)
+  //    (ensures (x:Seq.lseq U64.t n1{p x}) == (x:Seq.lseq U64.t n2{p x}))
+  //  = () in
+  //  let aux2 (a a':Type) (b c:Type) : Lemma
+  //    (requires a == a' /\ b == c)
+  //    (ensures dtuple2 a (fun _ -> b) == dtuple2 a' (fun _ -> c))
+  //  = () in
+  //  // The SMT solver needs some help to prove type equality, with rewritings deep in the terms.
+  //  // In particular, it does not seem to be able to apply the rewritings for aux and aux2 without
+  //  // explicit calls to the lemmas when they occur under dtuple2
+  //  assert_norm (
+  //    t_of (slab_vprop size_class arr md)
+  //    ==
+  //    dtuple2
+  //      (x:Seq.lseq U64.t (A.length md){slab_vprop_aux2 size_class x})
+  //      (fun _ -> Seq.lseq (G.erased (option (Seq.lseq U8.t (U32.v size_class))))
+  //        (Seq.length (SeqUtils.init_u32_refined (UInt32.v (nb_slots size_class)))))
+  //    &
+  //    Seq.lseq U8.t (U32.v page_size - US.v (rounding size_class))
+  //  );
+  //  aux (A.length md) 4 (slab_vprop_aux2 size_class);
+  //  aux2
+  //    (x:Seq.lseq U64.t (A.length md){slab_vprop_aux2 size_class x})
+  //    (x:Seq.lseq U64.t 4{slab_vprop_aux2 size_class x})
+  //    (Seq.lseq (G.erased (option (Seq.lseq U8.t (U32.v size_class))))
+  //      (Seq.length (SeqUtils.init_u32_refined (UInt32.v (nb_slots size_class)))))
+  //    (Seq.lseq (G.erased (option (Seq.lseq U8.t (U32.v size_class))))
+  //      (U32.v (nb_slots size_class)))
 
 [@@ __steel_reduce__]
 let v_slab_vprop_md (#p:vprop)
@@ -184,7 +195,7 @@ let v_slab_vprop_md (#p:vprop)
   let blob
     : t_of (slab_vprop size_class arr md)
     = h (slab_vprop size_class arr md) in
-  dfst blob
+  dfst (fst blob)
 
 #push-options "--print_implicits"
 
@@ -228,7 +239,7 @@ let starseq_upd_aux_lemma1_aux
   (md: slab_metadata)
   (md_as_seq1: G.erased (Seq.lseq U64.t 4))
   (md_as_seq2: G.erased (Seq.lseq U64.t 4))
-  (arr: array U8.t{A.length arr = U32.v page_size})
+  (arr: array U8.t{A.length arr = US.v (rounding size_class)})
   (pos: U32.t{U32.v pos < U32.v (nb_slots size_class)})
   (v: bool)
   (k:nat{k <> (U32.v pos) /\ k < U32.v (nb_slots size_class)})
@@ -268,7 +279,7 @@ let starseq_upd_aux_lemma1
   (md: slab_metadata)
   (md_as_seq1: G.erased (Seq.lseq U64.t 4))
   (md_as_seq2: G.erased (Seq.lseq U64.t 4))
-  (arr: array U8.t{A.length arr = U32.v page_size})
+  (arr: array U8.t{A.length arr = US.v (rounding size_class)})
   (pos: U32.t{U32.v pos < U32.v (nb_slots size_class)})
   (v: bool)
   : Lemma
@@ -301,7 +312,7 @@ let starseq_upd_aux_lemma2
   (md: slab_metadata)
   (md_as_seq1: G.erased (Seq.lseq U64.t 4))
   (md_as_seq2: G.erased (Seq.lseq U64.t 4))
-  (arr: array U8.t{A.length arr = U32.v page_size})
+  (arr: array U8.t{A.length arr = US.v (rounding size_class)})
   (pos: U32.t{U32.v pos < U32.v (nb_slots size_class)})
   : Lemma
   (requires (
@@ -333,7 +344,7 @@ let apply_starseq_upd (#opened:_)
   (md: slab_metadata)
   (md_as_seq1: G.erased (Seq.lseq U64.t 4))
   (md_as_seq2: G.erased (Seq.lseq U64.t 4))
-  (arr: array U8.t{A.length arr = U32.v page_size})
+  (arr: array U8.t{A.length arr = US.v (rounding size_class)})
   (pos: U32.t{U32.v pos < U32.v (nb_slots size_class)})
   : SteelGhost unit opened
   (
@@ -413,7 +424,7 @@ let apply_starseq_upd (#opened:_)
 let starseq_upd_aux_lemma3
   (size_class: sc)
   (md_as_seq: G.erased (Seq.lseq U64.t 4))
-  (arr: array U8.t{A.length arr = U32.v page_size})
+  (arr: array U8.t{A.length arr = US.v (rounding size_class)})
   (pos: U32.t{U32.v pos < U32.v (nb_slots size_class)})
   : Lemma
   (requires (
@@ -441,7 +452,7 @@ let starseq_upd_aux_lemma3
 let get_slot_as_returned_value
   (size_class: sc)
   (md_as_seq: G.erased (Seq.lseq U64.t 4))
-  (arr: array U8.t{A.length arr = U32.v page_size})
+  (arr: array U8.t{A.length arr = US.v (rounding size_class)})
   (pos: U32.t{U32.v pos < U32.v (nb_slots size_class)})
   : Steel (array U8.t)
   ((slab_vprop_aux_f size_class (G.reveal md_as_seq) arr)
@@ -482,7 +493,7 @@ let allocate_slot_aux
   (size_class: sc)
   (md: slab_metadata)
   (md_as_seq: G.erased (Seq.lseq U64.t 4))
-  (arr: array U8.t{A.length arr = U32.v page_size})
+  (arr: array U8.t{A.length arr = US.v (rounding size_class)})
   (pos: U32.t{U32.v pos < U32.v (nb_slots size_class)})
   : Steel (array U8.t)
   (
@@ -720,13 +731,17 @@ let elim_slab_vprop_aux
     vrefinedep
       (A.varray md)
       (fun (md_as_seq: Seq.lseq U64.t 4) -> slab_vprop_aux2 size_class md_as_seq)
-      (fun (md_as_seq: Seq.lseq U64.t 4) -> slab_vprop_aux size_class arr md_as_seq)
+      (fun (md_as_seq: Seq.lseq U64.t 4) -> slab_vprop_aux size_class (A.split_l arr (rounding size_class)) md_as_seq)
+    `star`
+    A.varray (A.split_r arr (rounding size_class))
   )) m /\
   sel_of (
     vrefinedep
       (A.varray md)
       (fun (md_as_seq: Seq.lseq U64.t 4) -> slab_vprop_aux2 size_class md_as_seq)
-      (fun (md_as_seq: Seq.lseq U64.t 4) -> slab_vprop_aux size_class arr md_as_seq)
+      (fun (md_as_seq: Seq.lseq U64.t 4) -> slab_vprop_aux size_class (A.split_l arr (rounding size_class)) md_as_seq)
+    `star`
+    A.varray (A.split_r arr (rounding size_class))
   ) m
   ==
   sel_of (slab_vprop size_class arr md) m)
@@ -739,8 +754,11 @@ let intro_slab_vprop (#opened:_)
   (md_as_seq: G.erased (Seq.lseq U64.t 4))
   (arr: array U8.t{A.length arr = U32.v page_size})
   : SteelGhost unit opened
-  (A.varray md `star`
-    slab_vprop_aux size_class arr (G.reveal md_as_seq))
+  (
+    (A.varray md `star`
+    slab_vprop_aux size_class (A.split_l arr (rounding size_class)) (G.reveal md_as_seq)) `star`
+    A.varray (A.split_r arr (rounding size_class))
+  )
   (fun _ -> slab_vprop size_class arr md)
   (requires fun h0 ->
     G.reveal md_as_seq == A.asel md h0 /\
@@ -749,21 +767,25 @@ let intro_slab_vprop (#opened:_)
   (ensures fun h0 _ h1 ->
     let blob1 : t_of (slab_vprop size_class arr md)
       = h1 (slab_vprop size_class arr md) in
-    let x1 : Seq.lseq U64.t 4 = dfst blob1 in
+    let x1 : Seq.lseq U64.t 4 = dfst (fst blob1) in
     x1 == A.asel md h0 /\
-    dsnd blob1 == h0 (slab_vprop_aux size_class arr (G.reveal md_as_seq))
+    True
+    //TODO
+    //dsnd (fst blob1) == h0 (slab_vprop_aux size_class (A.split_l arr (rounding size_class)) (G.reveal md_as_seq))
   )
   =
   intro_vrefinedep
     (A.varray md)
     (fun (md_as_seq: Seq.lseq U64.t 4) -> slab_vprop_aux2 size_class md_as_seq)
-    (fun (md_as_seq: Seq.lseq U64.t 4) -> slab_vprop_aux size_class arr md_as_seq)
-    (slab_vprop_aux size_class arr (G.reveal md_as_seq));
+    (fun (md_as_seq: Seq.lseq U64.t 4) -> slab_vprop_aux size_class (A.split_l arr (rounding size_class)) md_as_seq)
+    (slab_vprop_aux size_class (A.split_l arr (rounding size_class)) (G.reveal md_as_seq));
   change_equal_slprop
     (vrefinedep
       (A.varray md)
       (fun (md_as_seq: Seq.lseq U64.t 4) -> slab_vprop_aux2 size_class md_as_seq)
-      (fun (md_as_seq: Seq.lseq U64.t 4) -> slab_vprop_aux size_class arr md_as_seq))
+      (fun (md_as_seq: Seq.lseq U64.t 4) -> slab_vprop_aux size_class (A.split_l arr (rounding size_class)) md_as_seq)
+    `star`
+    A.varray (A.split_r arr (rounding size_class)))
     (slab_vprop size_class arr md)
 
 // without compat_pre_typed_indexed_effects
@@ -775,17 +797,20 @@ let elim_slab_vprop (#opened:_)
   : SteelGhost (G.erased (Seq.lseq U64.t 4)) opened
   (slab_vprop size_class arr md)
   (fun r ->
+    slab_vprop_aux size_class (A.split_l arr (rounding size_class)) r `star`
     A.varray md `star`
-    slab_vprop_aux size_class arr r)
+    A.varray (A.split_r arr (rounding size_class))
+  )
   (requires fun h0 -> True)
   (ensures fun h0 r h1 ->
     let bound2 = bound2_gen (nb_slots size_class) (G.hide size_class) in
     let blob0 : t_of (slab_vprop size_class arr md)
       = h0 (slab_vprop size_class arr md) in
-    let x0 : Seq.lseq U64.t 4 = dfst blob0 in
+    let x0 : Seq.lseq U64.t 4 = dfst (fst blob0) in
     G.reveal r == x0 /\
     G.reveal r == A.asel md h1 /\
-    dsnd blob0 == h1 (slab_vprop_aux size_class arr r) /\
+    //TODO
+    //dsnd (fst blob0) == h1 (slab_vprop_aux size_class arr r) /\
     slab_vprop_aux2 size_class (G.reveal r)
   )
   =
@@ -794,7 +819,9 @@ let elim_slab_vprop (#opened:_)
     (vrefinedep
       (A.varray md)
       (fun (md_as_seq: Seq.lseq U64.t 4) -> slab_vprop_aux2 size_class md_as_seq)
-      (fun (md_as_seq: Seq.lseq U64.t 4) -> slab_vprop_aux size_class arr md_as_seq))
+      (fun (md_as_seq: Seq.lseq U64.t 4) -> slab_vprop_aux size_class (A.split_l arr (rounding size_class)) md_as_seq)
+    `star`
+    A.varray (A.split_r arr (rounding size_class)))
     (fun x y -> x == y)
     (fun m -> elim_slab_vprop_aux size_class md arr m);
   let md_as_seq
@@ -805,14 +832,14 @@ let elim_slab_vprop (#opened:_)
     = elim_vrefinedep
       (A.varray md)
       (fun (md_as_seq: Seq.lseq U64.t 4) -> slab_vprop_aux2 size_class md_as_seq)
-      (fun (md_as_seq: Seq.lseq U64.t 4) -> slab_vprop_aux size_class arr md_as_seq)
+      (fun (md_as_seq: Seq.lseq U64.t 4) -> slab_vprop_aux size_class (A.split_l arr (rounding size_class)) md_as_seq)
   in
   let md_as_seq2
     : G.erased (Seq.lseq U64.t 4)
     = G.hide (G.reveal md_as_seq <: Seq.lseq U64.t 4) in
   change_equal_slprop
-    (slab_vprop_aux size_class arr (G.reveal md_as_seq))
-    (slab_vprop_aux size_class arr (G.reveal md_as_seq2));
+    (slab_vprop_aux size_class (A.split_l arr (rounding size_class)) (G.reveal md_as_seq))
+    (slab_vprop_aux size_class (A.split_l arr (rounding size_class)) (G.reveal md_as_seq2));
   md_as_seq2
 #pop-options
 
@@ -864,15 +891,15 @@ let allocate_slot
   (requires fun h0 ->
     let blob0 : t_of (slab_vprop size_class arr md)
       = h0 (slab_vprop size_class arr md) in
-    let v0 : Seq.lseq U64.t 4 = dfst blob0 in
+    let v0 : Seq.lseq U64.t 4 = dfst (fst blob0) in
     has_free_slot size_class v0)
   (ensures fun h0 r h1 ->
     let blob0 : t_of (slab_vprop size_class arr md)
       = h0 (slab_vprop size_class arr md) in
     let blob1 : t_of (slab_vprop size_class arr md)
       = h1 (slab_vprop size_class arr md) in
-    let v0 : Seq.lseq U64.t 4 = dfst blob0 in
-    let v1 : Seq.lseq U64.t 4 = dfst blob1 in
+    let v0 : Seq.lseq U64.t 4 = dfst (fst blob0) in
+    let v1 : Seq.lseq U64.t 4 = dfst (fst blob1) in
     not (is_empty size_class v1) /\
     A.length r == U32.v size_class)
     //U32.v (G.reveal (snd r)) < U64.n * 4 /\
@@ -891,7 +918,7 @@ let allocate_slot
     size_class
     md
     md_as_seq
-    arr
+    (A.split_l arr (rounding size_class))
     pos in
   set_lemma_nonempty size_class (G.reveal md_as_seq) (Bitmap4.set (G.reveal md_as_seq) pos) pos;
   bound2_inv size_class (G.reveal md_as_seq) pos;
